Add concrete interpretation of LSSA programs.

src/LoopFormalization/LSSA.v
@@ -117,7 +117,7 @@ Inductive term_step: Program -> Term -> RegisterMap -> (bbid * RegisterMap)
 (* The semantics of a list of instructions *)
 Inductive inst_list_denotation: (list Inst) -> RegisterMap -> RegisterMap -> Prop :=
 | EmptyInstListStep (R: RegisterMap) : inst_list_denotation nil R R
-| ConstInstListStep (i: Inst) (l: list Inst) (R R' R'': RegisterMap) :
+| ConsInstListStep (i: Inst) (l: list Inst) (R R' R'': RegisterMap) :
     inst_step i R R' -> inst_list_denotation l R' R'' ->
     inst_list_denotation (i::l) R R''.
 
@@ -128,25 +128,234 @@ Inductive bb_denotation: Program -> BasicBlock -> RegisterMap -> (bbid * Registe
 
 (* The semantics of a program *)
 Inductive program_denotation: Program -> Program -> (bbid * RegisterMap) -> (bbid * RegisterMap) -> Prop :=
-| BBInDenot (p: Program) (out_id: bbid) (bb: BasicBlock) (R R': RegisterMap):
-    bb_denotation p bb R (out_id, R') ->
-    program_denotation p (BB bb) (bb.1.1.1, R) (out_id, R')
-| BBNotInDenot (p: Program) (in_id: bbid) (bb: BasicBlock) (R: RegisterMap):
-    ~~(bb.1.1.1 =? in_id)%string ->
-    program_denotation p (BB bb) (in_id, R) (in_id, R)
+| BBInDenot (p: Program) (out_id bb_id: bbid) (params: list vid) (insts: list Inst)
+            (term: Term) (R R': RegisterMap):
+    bb_denotation p (bb_id, params, insts, term) R (out_id, R') ->
+    program_denotation p (BB (bb_id, params, insts, term)) (bb_id, R) (out_id, R')
+| BBNotInDenot (p: Program) (in_id bb_id: bbid) (params: list vid) (insts: list Inst)
+            (term: Term) (R R': RegisterMap):
+    ~~(bb_id =? in_id)%string ->
+    program_denotation p (BB (bb_id, params, insts, term)) (in_id, R) (in_id, R)
 | DAGDenot (p p1 p2: Program) (R R' R'': RegisterMap) (id id' id'': bbid):
     program_denotation p p1 (id, R) (id', R') ->
     program_denotation p p2 (id', R') (id'', R'') ->
     program_denotation p (DAG p1 p2) (id, R) (id'', R'')
-| LoopNotInDenot (p: Program) (header: BasicBlock) (body: option Program) (id: bbid) (R: RegisterMap):
-    ~~(header.1.1.1 =? id)%string ->
-    program_denotation p (Loop header body) (id, R) (id, R)
-| LoopSingleInDenot (p: Program) (header: BasicBlock) (id1 id2: bbid) (R0 R1 R2: RegisterMap):
-    bb_denotation p header R0 (id1, R1) ->
-    program_denotation p (Loop header None) (id1, R1) (id2, R2) ->
-    program_denotation p (Loop header None) (header.1.1.1, R0) (id2, R2)
-| LoopInDenot (p body: Program) (header: BasicBlock) (id1 id2 id3: bbid) (R0 R1 R2 R3: RegisterMap):
-    bb_denotation p header R0 (id1, R1) ->
+| LoopNotInDenot (p: Program) (header_id: bbid) (params: list vid) (insts: list Inst)
+                 (term: Term) (body: option Program) (id: bbid) (R: RegisterMap):
+    ~~(header_id =? id)%string ->
+    program_denotation p (Loop (header_id, params, insts, term) body) (id, R) (id, R)
+| LoopSingleInDenot (p: Program) (header_id: bbid) (params: list vid) (insts: list Inst)
+                    (term: Term) (id1 id2: bbid) (R0 R1 R2: RegisterMap):
+    bb_denotation p (header_id, params, insts, term) R0 (id1, R1) ->
+    program_denotation p (Loop (header_id, params, insts, term) None) (id1, R1) (id2, R2) ->
+    program_denotation p (Loop (header_id, params, insts, term) None) (header_id, R0) (id2, R2)
+| LoopInDenot (p body: Program) (header_id: bbid) (params: list vid) (insts: list Inst)
+              (term: Term) (id1 id2 id3: bbid) (R0 R1 R2 R3: RegisterMap):
+    bb_denotation p (header_id, params, insts, term) R0 (id1, R1) ->
     program_denotation p body (id1, R1) (id2, R2) ->
-    program_denotation p (Loop header (Some body)) (id2, R2) (id3, R3) ->
-    program_denotation p (Loop header (Some body)) (header.1.1.1, R0) (id3, R3).
+    program_denotation p (Loop (header_id, params, insts, term) (Some body)) (id2, R2) (id3, R3) ->
+    program_denotation p (Loop (header_id, params, insts, term) (Some body)) (header_id, R0) (id3, R3).
+
+
+Definition interpret_instruction (inst: Inst) (R: RegisterMap) :=
+  match inst with
+  | Const v c => (v !-> c; R)
+  | BinOp v opc op1 op2 _ _ => (v !-> bin_op_eval opc (R op1) (R op2); R)
+  end.
+
+Theorem interpret_instruction_spec :
+  forall inst R, inst_step inst R (interpret_instruction inst R).
+Proof.
+  move => inst R.
+  case inst; constructor.
+Qed.
+
+Definition interpret_term (p: Program) (t: Term) (R: RegisterMap) :=
+  match t with
+  | Br bb params => (bb, affect_variables R (get_inputs p bb) params)
+  | BrC c bbT paramsT bbF paramsF =>
+    if R c =? 0 then
+      (bbF, affect_variables R (get_inputs p bbF) paramsF)
+    else
+      (bbT, affect_variables R (get_inputs p bbT) paramsT)
+  end.
+
+Theorem interpret_term_spec :
+  forall p t R, term_step p t R (interpret_term p t R).
+Proof.
+  move => p t R.
+  case t => [ bb params | c bbT paramsT bbF paramsF /=].
+  - constructor.
+  - case (Z.eqb_spec (R c) 0); by constructor.
+Qed.
+
+Fixpoint interpret_inst_list (l: list Inst) (R: RegisterMap) :=
+  match l with
+  | nil => R
+  | inst::l' => interpret_inst_list l' (interpret_instruction inst R)
+  end.
+
+Theorem interpret_inst_list_spec :
+  forall l R, inst_list_denotation l R (interpret_inst_list l R).
+Proof.
+  elim => [ | i l0 Hind R /= ].
+  - constructor.
+  - eapply ConsInstListStep.
+    + by apply interpret_instruction_spec.
+    + by [].
+Qed.
+
+Definition interpret_bb (p: Program) (bb: BasicBlock) (R: RegisterMap) :=
+  interpret_term p bb.2 (interpret_inst_list bb.1.2 R).
+
+Theorem interpret_bb_spec :
+  forall p bb R, bb_denotation p bb R (interpret_bb p bb R).
+Proof.
+  move => p [[[bb_id params] insts] term] R.
+  move H: (interpret_bb p (bb_id, params, insts, term) R) => bbR'.
+  case: bbR' H => a b Hbb.
+  eapply BBDenot.
+  - apply interpret_inst_list_spec.
+  - rewrite -Hbb.
+    rewrite /interpret_bb /=.
+      by apply interpret_term_spec.
+Qed.
+
+Fixpoint interpret_program (fuel: nat) (p sub_p: Program) (id: bbid) (R: RegisterMap) :=
+  if fuel is S fuel' then
+    match sub_p with
+    | BB bb =>
+      if (id =? bb.1.1.1)%string then
+        Some (interpret_bb p bb R)
+      else
+        Some (id, R)
+    | DAG p1 p2 =>
+      if interpret_program fuel' p p1 id R is Some (id', R') then
+        interpret_program fuel' p p2 id' R'
+      else
+        None
+    | Loop h None =>
+      if (id =? h.1.1.1)%string then
+        let (id', R') := interpret_bb p h R in
+        interpret_program fuel' p (Loop h None) id' R'
+      else
+        Some (id, R)
+    | Loop h (Some body) =>
+      if (id =? h.1.1.1)%string then
+        let (id', R') := interpret_bb p h R in
+        if interpret_program fuel' p body id' R' is Some (id'', R'') then
+          interpret_program fuel' p (Loop h (Some body)) id'' R''
+        else
+          None
+      else
+        Some (id, R)
+    end
+  else
+    None.
+
+Theorem interpret_program_spec :
+  forall fuel p sub_p id R id' R',
+    Some (id', R') = interpret_program fuel p sub_p id R ->
+    program_denotation p sub_p (id, R) (id', R').
+Proof.
+  elim => [ p sub_p id R id' R' Hsome // | n Hind p sub_p id R id' R'].
+  case sub_p => [ [[[header_id params] insts] term] [ body | ] /= | p1 p2 /= HDAG | [[[bb_id params] insts] term]].
+  - case_eq (id =? header_id)%string; last first.
+    + move => Hne [-> ->].
+      apply LoopNotInDenot.
+      by rewrite eqb_sym Hne.
+    + move => /eqb_eq -> Hinterpret.
+      move Hbb_interpret: (interpret_bb p (header_id, params, insts, term) R) => bb_interpret.
+      move: bb_interpret => [id_bb_interpret R_bb_interpret] in Hbb_interpret.
+      rewrite Hbb_interpret in Hinterpret.
+      move: Hinterpret.
+      case_eq (interpret_program n p body id_bb_interpret R_bb_interpret) => [ [p0_id p0R] Hinterpret HSome | //].
+      eapply LoopInDenot with (id1 := id_bb_interpret) (R1 := R_bb_interpret) (id2 := p0_id) (R2 := p0R).
+      * rewrite -Hbb_interpret.
+        by apply interpret_bb_spec.
+      * by apply Hind.
+      * by apply Hind.
+  - case_eq (id =? header_id)%string => [ /eqb_eq -> Hinterpret | Hne [-> ->]].
+    + move Hp0: (interpret_bb p (header_id, params, insts, term) R) => [p0_id p0_R].
+      apply LoopSingleInDenot with (id1 := p0_id) (R1 := p0_R).
+      * rewrite -Hp0.
+          by apply interpret_bb_spec.
+      * rewrite Hp0 in Hinterpret.
+          by apply Hind.
+    + apply LoopNotInDenot.
+      by rewrite eqb_sym Hne.
+  - case (interpret_program n p p1 id R) eqn:Hp1 in HDAG.
+    move: p0 => [p0_id p0_R] in HDAG Hp1.
+    eapply DAGDenot.
+    + apply Hind.
+      symmetry.
+        by apply Hp1.
+    + by apply Hind.
+    + by [].
+  - rewrite /interpret_program /=.
+    case (eqb_spec id bb_id)%string => [-> [HBB] | /eqb_spec Hne [-> ->]].
+    + apply BBInDenot.
+      rewrite HBB.
+      apply interpret_bb_spec.
+    + apply BBNotInDenot.
+      apply R.
+        by rewrite eqb_sym.
+Qed.
+
+Section Example.
+
+  Definition entry_bb := ("entry", @nil string,
+                          (Const "zero" 0)::(Const "one" 1)::nil,
+                          (Br "loop" ("zero"::nil))).
+
+  Definition y_ne_x : "y" <> "x".
+  Proof.
+      by apply eqb_neq.
+  Qed.
+
+  Definition y_ne_one : "y" <> "one".
+  Proof.
+      by apply eqb_neq.
+  Qed.
+
+  Definition c_ne_y : "c" <> "y".
+  Proof.
+      by apply eqb_neq.
+  Qed.
+
+  Definition c_ne_one : "c" <> "one".
+  Proof.
+      by apply eqb_neq.
+  Qed.
+
+
+  Definition loop_header := ("loop", "x"::nil,
+                             (BinOp "y" OpAdd "x" "one" y_ne_x y_ne_one)::
+                             (BinOp "c" OpLe "y" "one" c_ne_y c_ne_one)::nil,
+                             (BrC "c" "loop" ("y"::nil) "exit" ("y"::nil))).
+
+  Definition loop := Loop loop_header None.
+
+  Definition exit_bb := ("exit", "exitvalue"::nil, @nil Inst, (Br "finished" nil)).
+
+  Definition program := DAG (BB entry_bb) (DAG loop (BB exit_bb)).
+
+  Definition input := ("entry", (_ !-> 0)).
+
+  Transparent eval_map.
+
+  Example program_may_terminate :
+    forall R, exists R', program_denotation program program ("entry", R) ("finished", R').
+  Proof.
+    move => R.
+    move Hfinal_state: (interpret_program 10%nat program program "entry" R) => final.
+    move: (interpret_program_spec 10 program program "entry" R).
+    rewrite Hfinal_state.
+    move: final Hfinal_state => [[id' R'] Hfinal | // ].
+    move => /(_ id' R' (eq_refl _)) Hgoal.
+    exists R'.
+    compute in Hfinal.
+    by move: Hfinal => [-> _].
+  Qed.
+
+End Example.
